DenotSem/Deterministic.thy
@@ -22,7 +22,7 @@ lemma merge_inter_equiv: "\<lbrakk> A ~ B; B \<approx> B' \<rbrakk> \<Longrighta
     apply force
   done
   
-lemma fold_merge_equiv_fold_meet: fixes xs::"ty list"
+lemma fold_merge_equiv_fold_meet_aux: fixes xs::"ty list"
   assumes c_xs: "\<forall>v1 v2. {v1,v2} \<subseteq> set xs \<longrightarrow> v1 ~ v2" and x_xp: "x \<approx> x'" and
     x_xs: "\<forall>v. v \<in> set xs \<longrightarrow> x ~ v" and wf_xs: "\<forall>v. v \<in> set xs \<longrightarrow> wf_ty v" and wf_x: "wf_ty x" 
   shows "fold merge xs x \<approx> fold op \<sqinter> xs x'"
@@ -46,33 +46,140 @@ next
     using Cons.IH[of "merge a x" "a \<sqinter> x'"] 1 2 3 4 5 by blast  
   then show ?case by simp
 qed
-    
-    
-lemma consistent_app: assumes f1_f2: "f1 ~ f2" and v1_v2: "v1 ~ v2" and 
-  f1_v1: "v1' \<in> f1 \<bullet> v1"  and f2_v2: "v2' \<in> f2 \<bullet> v2" 
-shows "v1' ~ v2'"
+
+lemma merge_list_equiv_meet_list: fixes xs::"ty list"
+  assumes c_xs: "\<forall>v1 v2. {v1,v2} \<subseteq> set xs \<longrightarrow> v1 ~ v2" and wf_xs: "\<forall>v. v \<in> set xs \<longrightarrow> wf_ty v" 
+    and xs_ne: "xs \<noteq> []"
+  shows "\<Prod>xs \<approx> \<Sqinter>xs"
 proof -
-  have f1_v11: "f1 <: v1 \<rightarrow> v1'" using f1_v1 by simp
-  have f2_v22: "f2 <: v2 \<rightarrow> v2'" using f2_v2 by simp
-
-  obtain \<Gamma>1 where g1_ne: "\<Gamma>1 \<noteq> []" and "all_funs \<Gamma>1" and g1_f1: "set \<Gamma>1 \<subseteq> atoms f1" and
-    v1_g1: "\<forall>v v'. v\<rightarrow>v' \<in> set \<Gamma>1 \<longrightarrow> v1 <: v" and g1_v1p: "\<Sqinter>(map cod \<Gamma>1) <: v1'"
-    using f1_v11 sub_fun_any_inv_atoms[of f1 v1 v1'] by blast
-    
-  obtain \<Gamma>2 where g2_ne: "\<Gamma>2 \<noteq> []" and "all_funs \<Gamma>2" and g2_f2: "set \<Gamma>2 \<subseteq> atoms f2" and
-    v2_g2: "\<forall>v v'. v\<rightarrow>v' \<in> set \<Gamma>2 \<longrightarrow> v2 <: v" and g2_v2p: "\<Sqinter>(map cod \<Gamma>2) <: v2'"
-    using f2_v22 sub_fun_any_inv_atoms[of f2 v2 v2'] by blast
-
-  { fix a b c d
-    assume ab_g1: "a\<rightarrow>b \<in> set \<Gamma>1" and cd_g2: "c\<rightarrow>d \<in> set \<Gamma>2"
+  obtain x xs' where xs: "xs = x#xs'" using xs_ne by (cases xs) auto      
+  have 1: "\<forall>v1 v2. {v1,v2} \<subseteq> set xs' \<longrightarrow> v1 ~ v2" using c_xs xs by auto
+  have 2: "x \<approx> x" by auto
+  have 3: "\<forall>v. v \<in> set xs' \<longrightarrow> x ~ v" using c_xs xs by auto
+  have 4: "\<forall>v. v \<in> set xs' \<longrightarrow> wf_ty v" using wf_xs xs by auto
+  have 5: "wf_ty x" using wf_xs xs by auto
+  have "fold merge xs' x \<approx> fold op \<sqinter> xs' x" 
+    using 1 2 3 4 5 fold_merge_equiv_fold_meet_aux[of xs' x x] by blast
+  then show ?thesis using xs merge_list_def meet_list_def by simp
+qed
+  
+lemma consis_codomain:
+  fixes a b c d
+  assumes ab_g1: "a\<rightarrow>b \<in> set \<Gamma>1" and cd_g2: "c\<rightarrow>d \<in> set \<Gamma>2" and
+    v1_g1: "\<forall>v v'. v\<rightarrow>v' \<in> set \<Gamma>1 \<longrightarrow> v1 <: v" and
+    v2_g2: "\<forall>v v'. v\<rightarrow>v' \<in> set \<Gamma>2 \<longrightarrow> v2 <: v" and
+    v1_v2: "v1 ~ v2" and f1_f2: "f1 ~ f2" and
+    g1_f1: "set \<Gamma>1 \<subseteq> atoms f1" and g2_f2: "set \<Gamma>2 \<subseteq> atoms f2"
+  shows "b ~ d"
+proof -    
     have v1_a: "v1 <: a" using v1_g1 ab_g1 by blast 
     have v2_c: "v2 <: c" using v2_g2 cd_g2 by blast
     have a_c: "a ~ c" using v1_a v2_c v1_v2 consis_le by blast        
     have ab_cd: "a\<rightarrow>b ~ c\<rightarrow>d"
       using ab_g1 cd_g2 g1_f1 g2_f2 f1_f2 consis_atoms by blast
-    have "b ~ d" using ab_cd a_c by simp
-  }
-  then have "\<Sqinter>(map cod \<Gamma>1) ~ \<Sqinter>(map cod \<Gamma>2)" sorry
+    show "b ~ d" using ab_cd a_c by simp 
+qed
+
+lemma all_fun_ex: "\<lbrakk> all_funs \<Gamma>; x \<in> set \<Gamma>; \<And> a b. \<lbrakk> x = a \<rightarrow> b \<rbrakk> \<Longrightarrow> P \<rbrakk> \<Longrightarrow> P"
+  apply (cases x) apply auto done
+
+lemma all_fun_ex_dom: "\<lbrakk> all_funs \<Gamma>; y \<in> set (map cod \<Gamma>) \<rbrakk> \<Longrightarrow> \<exists>x. x\<rightarrow>y \<in> set \<Gamma>"
+  apply (induction \<Gamma> arbitrary: y)
+  apply force
+  apply simp apply (erule disjE) 
+   apply simp apply (case_tac a) apply force apply force apply force
+  apply blast
+  done
+    
+lemma consistent_app: assumes f1_f2: "f1 ~ f2" and v1_v2: "v1 ~ v2" and 
+  f1_v1: "v1' \<in> f1 \<bullet> v1"  and f2_v2: "v2' \<in> f2 \<bullet> v2" and
+  wf_f1: "wf_ty f1" and wf_f2: "wf_ty f2" and wf_v1: "wf_ty v1" and wf_v2: "wf_ty v2"
+shows "v1' ~ v2'"
+proof -
+  have f1_v11: "f1 <: v1 \<rightarrow> v1'" using f1_v1 by simp
+  have f2_v22: "f2 <: v2 \<rightarrow> v2'" using f2_v2 by simp
+      
+  obtain \<Gamma>1 where g1_ne: "\<Gamma>1 \<noteq> []" and af_g1: "all_funs \<Gamma>1" and g1_f1: "set \<Gamma>1 \<subseteq> atoms f1" and
+    v1_g1: "\<forall>v v'. v\<rightarrow>v' \<in> set \<Gamma>1 \<longrightarrow> v1 <: v" and g1_v1p: "\<Sqinter>(map cod \<Gamma>1) <: v1'"
+    using f1_v11 sub_fun_any_inv_atoms[of f1 v1 v1'] by blast
+  let ?C1 = "map cod \<Gamma>1"     
+  obtain \<Gamma>2 where g2_ne: "\<Gamma>2 \<noteq> []" and af_g2: "all_funs \<Gamma>2" and g2_f2: "set \<Gamma>2 \<subseteq> atoms f2" and
+    v2_g2: "\<forall>v v'. v\<rightarrow>v' \<in> set \<Gamma>2 \<longrightarrow> v2 <: v" and g2_v2p: "\<Sqinter>(map cod \<Gamma>2) <: v2'"
+    using f2_v22 sub_fun_any_inv_atoms[of f2 v2 v2'] by blast
+  let ?C2 = "map cod \<Gamma>2"
+
+  have wf_c1: "\<forall>v. v \<in> set ?C1 \<longrightarrow> wf_ty v"
+    using g1_f1 wf_f1 af_g1 apply auto
+    apply (erule all_fun_ex) apply blast apply simp using wf_atoms apply auto done
+  have wf_c2: "\<forall>v. v \<in> set ?C2 \<longrightarrow> wf_ty v"
+    using g2_f2 wf_f2 af_g2 apply auto
+    apply (erule all_fun_ex) apply blast apply simp using wf_atoms apply auto done
+  have c_c1: "\<forall>v1' v2'. {v1',v2'} \<subseteq> set ?C1 \<longrightarrow> v1' ~ v2'"
+  proof clarify
+    fix v1' v2' assume 1: "{v1',v2'} \<subseteq> set ?C1"        
+    have v1_c1: "v1' \<in> set ?C1" using 1 by blast 
+    have v2_c1: "v2' \<in> set ?C1" using 1 by blast
+    obtain d1 where v11_g1: "d1\<rightarrow>v1' \<in> set \<Gamma>1" using v1_c1 af_g1 all_fun_ex_dom[of \<Gamma>1 v1'] by blast
+    obtain d2 where v22_g1: "d2\<rightarrow>v2' \<in> set \<Gamma>1" using v2_c1 af_g1 all_fun_ex_dom[of \<Gamma>1 v2'] by blast        
+    show "v1' ~ v2'"
+      apply (rule consis_codomain[of d1 v1' \<Gamma>1 d2 v2' \<Gamma>1 v1 v1 f1 f1])
+      using v11_g1 v22_g1 v1_g1 consis_refl wf_v1 wf_f1 g1_f1 by auto   
+  qed
+  have c_c2: "\<forall>v1' v2'. {v1',v2'} \<subseteq> set ?C2 \<longrightarrow> v1' ~ v2'"
+  proof clarify
+    fix v1' v2' assume 1: "{v1',v2'} \<subseteq> set ?C2"        
+    have v1_c1: "v1' \<in> set ?C2" using 1 by blast 
+    have v2_c1: "v2' \<in> set ?C2" using 1 by blast
+    obtain d1 where v11_g2: "d1\<rightarrow>v1' \<in> set \<Gamma>2" using v1_c1 af_g2 all_fun_ex_dom[of \<Gamma>2 v1'] by blast
+    obtain d2 where v22_g2: "d2\<rightarrow>v2' \<in> set \<Gamma>2" using v2_c1 af_g2 all_fun_ex_dom[of \<Gamma>2 v2'] by blast        
+    show "v1' ~ v2'"
+      apply (rule consis_codomain[of d1 v1' \<Gamma>2 d2 v2' \<Gamma>2 v2 v2 f2 f2])
+      using v11_g2 v22_g2 v2_g2 consis_refl wf_v2 wf_f2 g2_f2 by auto   
+  qed
+  have c1_c2: "\<Prod>?C1 ~ \<Prod>?C2"
+  proof (rule consis_merge_list)
+    show "\<forall>v1 v2. {v1, v2} \<subseteq> set ?C1 \<union> set ?C2 \<longrightarrow> v1 ~ v2"
+    proof clarify
+      fix v1' v2' assume 1: "{v1',v2'} \<subseteq> set ?C1 \<union> set ?C2"        
+      { assume v1_c1: "v1' \<in> set ?C1" and v2_c1: "v2' \<in> set ?C1"
+        have "v1' ~ v2'" using v1_c1 v2_c1 c_c1 by blast
+      } moreover {
+        assume v1_c1: "v1' \<in> set ?C1" and v2_c2: "v2' \<in> set ?C2"
+        obtain d1 where v11_g1: "d1\<rightarrow>v1' \<in> set \<Gamma>1" using v1_c1 af_g1 all_fun_ex_dom[of \<Gamma>1 v1'] by blast
+        obtain d2 where v22_g2: "d2\<rightarrow>v2' \<in> set \<Gamma>2" using v2_c2 af_g2 all_fun_ex_dom[of \<Gamma>2 v2'] by blast        
+        have "v1' ~ v2'" 
+          apply (rule consis_codomain)
+          using v11_g1 apply blast using v22_g2 apply blast using v1_g1 apply blast
+          using v2_g2 apply blast using v1_v2 apply blast using f1_f2 apply blast
+          using g1_f1 apply blast using g2_f2 apply blast done          
+      } moreover {
+        assume v1_c2: "v1' \<in> set ?C2" and v2_c1: "v2' \<in> set ?C1"
+        obtain d1 where v11_g2: "d1\<rightarrow>v1' \<in> set \<Gamma>2" using v1_c2 af_g2 all_fun_ex_dom[of \<Gamma>2 v1'] by blast
+        obtain d2 where v22_g1: "d2\<rightarrow>v2' \<in> set \<Gamma>1" using v2_c1 af_g1 all_fun_ex_dom[of \<Gamma>1 v2'] by blast        
+        have "v1' ~ v2'" 
+          apply (rule consis_codomain)
+          using v11_g2 apply blast using v22_g1 apply blast using v2_g2 apply blast
+          using v1_g1 apply blast using v1_v2 consis_sym apply blast
+          apply (rule consis_sym) using f1_f2 apply blast using g2_f2 apply blast           
+          using g1_f1 apply blast done        
+      } moreover {
+        assume v1_c2: "v1' \<in> set ?C2" and v2_c2: "v2' \<in> set ?C2"
+        have "v1' ~ v2'" using v1_c2 v2_c2 c_c2 g2_ne by auto 
+      } ultimately show "v1' ~ v2'" using 1 by blast
+    qed      
+  next
+    show "\<forall>v. v \<in> set ?C1 \<longrightarrow> wf_ty v" using wf_c1 by blast
+  next
+    show "\<forall>v. v \<in> set ?C2 \<longrightarrow> wf_ty v" using wf_c2 by blast
+  next
+    show "map cod \<Gamma>1 \<noteq> []" using g1_ne by simp
+  next
+    show "map cod \<Gamma>2 \<noteq> []" using g2_ne by simp
+  qed
+  have c1_c1: "\<Prod>?C1 \<approx> \<Sqinter>?C1" using merge_list_equiv_meet_list wf_c1 c_c1 g1_ne by auto
+  have c2_c2: "\<Prod>?C2 \<approx> \<Sqinter>?C2" using merge_list_equiv_meet_list wf_c2 c_c2 g2_ne by auto    
+  have "\<Sqinter>?C1 ~ \<Sqinter>?C2" using c1_c1 c1_c2 c2_c2 
+      using consis_le ty_equiv_def by auto 
   then show ?thesis using g1_v1p g2_v2p consis_le by blast
 qed
   
